rename

StandardLibrary/src/String.dfy
@@ -10,7 +10,7 @@ module StandardLibrary.String {
   import opened MemoryMath
   export provides Int2String, Base10Int2String, HasSubString, Wrappers, UInt,
                   HasSubStringPos, SearchAndReplace, SearchAndReplacePos, SearchAndReplaceAll,
-                  SearchAndReplacePosNot, SearchAndReplaceAllNot, AlphaNumeric, AlphaNumericUnder
+                  SearchAndReplacePosWhole, SearchAndReplaceAllWhole, AlphaNumeric, AlphaNumericUnder
 
   const Base10: seq<char> := ['0', '1', '2', '3', '4', '5', '6', '7', '8', '9']
 
@@ -63,18 +63,8 @@ module StandardLibrary.String {
     returns (o : seq<T>)
     requires 0 < |old_str|
   {
-    var old_pos := HasSubString(source, old_str);
-    if old_pos.None? {
-      return source;
-    } else {
-      SequenceIsSafeBecauseItIsInMemory(source);
-      SequenceIsSafeBecauseItIsInMemory(old_str);
-      ValueIsSafeBecauseItIsInMemory(old_pos.value);
-      var pos : uint64 := old_pos.value as uint64;
-      var source_len : uint64 := |source| as uint64;
-      var old_str_len : uint64 := |old_str| as uint64;
-      return source[..pos] + new_str + source[pos+old_str_len..];
-    }
+    var x := SearchAndReplacePos(source, old_str, new_str, 0);
+    return x.0;
   }
 
   // Replace first occurrence of old_str after pos in source with new_str and return the result.
@@ -103,28 +93,28 @@ module StandardLibrary.String {
     }
   }
 
-  predicate method BadStart<T(==)>(source : seq<T>, pos : uint64, forbid : seq<T>)
+  predicate method BadStart<T(==)>(source : seq<T>, pos : uint64, chars : seq<T>)
     requires pos as nat <= |source|
   {
     if pos == 0 then
       false
     else
-      source[pos-1] in forbid
+      source[pos-1] in chars
   }
 
-  predicate method BadEnd<T(==)>(source : seq<T>, pos : uint64, match_len : uint64, forbid : seq<T>) {
+  predicate method BadEnd<T(==)>(source : seq<T>, pos : uint64, match_len : uint64, chars : seq<T>) {
     SequenceIsSafeBecauseItIsInMemory(source);
     var source_len : uint64 := |source| as uint64;
     if Add(pos, match_len) >= source_len then
       false
     else
-      source[pos+match_len] in forbid
+      source[pos+match_len] in chars
 
   }
-  predicate method BadMatch<T(==)>(source : seq<T>, pos : uint64, match_len : uint64, forbid : seq<T>)
+  predicate method BadMatch<T(==)>(source : seq<T>, pos : uint64, match_len : uint64, chars : seq<T>)
     requires pos as nat <= |source|
   {
-    BadStart(source, pos, forbid) || BadEnd(source, pos, match_len, forbid)
+    BadStart(source, pos, chars) || BadEnd(source, pos, match_len, chars)
   }
 
   const AlphaNumeric      : string := "abcdefghijklmnopqrstuvwxyzABCDEFGHIJKLMNOPQRSTUVWXYZ0123456789"
@@ -133,8 +123,8 @@ module StandardLibrary.String {
   // Replace first occurrence of old_str after pos in source with new_str and return the result.
   // If old_str does not exist in source, the source is returned unchanged
   // second value in output is None if old_str not found, otherwise it points just after the replaced value
-  // a match only counts if the character before or after is not in forbid
-  method SearchAndReplacePosNot<T(==)>(source: seq<T>, old_str: seq<T>, new_str: seq<T>, xpos : uint64, forbid : seq<T>)
+  // a match only counts if the character before or after is not in chars
+  method SearchAndReplacePosWhole<T(==)>(source: seq<T>, old_str: seq<T>, new_str: seq<T>, xpos : uint64, chars : seq<T>)
     returns (o : (seq<T>, Option<uint64>))
     requires xpos as nat <= |source|
     requires 0 < |old_str|
@@ -150,7 +140,7 @@ module StandardLibrary.String {
       var old_pos := HasSubStringPos(source, old_str, pos);
       if old_pos.None? {
         return (source, None);
-      } else if BadMatch(source, old_pos.value, old_str_len, forbid) {
+      } else if BadMatch(source, old_pos.value, old_str_len, chars) {
         pos := old_pos.value + 1;
       } else {
         SequenceIsSafeBecauseItIsInMemory(source);
@@ -165,6 +155,18 @@ module StandardLibrary.String {
     return (source, None); // not really needed, but Dafny is dumb
   }
 
+  // Replace first occurrence of old_str after pos in source with new_str and return the result.
+  // If old_str does not exist in source, the source is returned unchanged
+  // second value in output is None if old_str not found, otherwise it points just after the replaced value
+  // a match only counts if the character before or after is not in chars
+  method SearchAndReplaceWhole<T(==)>(source: seq<T>, old_str: seq<T>, new_str: seq<T>, chars : seq<T>)
+    returns (o : (seq<T>, Option<uint64>))
+    requires 0 < |old_str|
+    ensures o.1.Some? ==> |o.0| - o.1.value as nat < |source| as nat
+    ensures o.1.Some? ==> o.1.value as nat <= |o.0|
+  {
+    o := SearchAndReplacePosWhole(source, old_str, new_str, 0, chars);
+  }
 
   // Replace all occurrences of old_str in source with new_str and return the result.
   // If old_str does not exist in source, the source is returned unchanged
@@ -193,8 +195,8 @@ module StandardLibrary.String {
   // Replace all occurrences of old_str in source with new_str and return the result.
   // If old_str does not exist in source, the source is returned unchanged
   // safe to use if new_str contains old_str
-  // a match only counts if the character before or after is not in forbid
-  method SearchAndReplaceAllNot<T(==)>(source_in: seq<T>, old_str: seq<T>, new_str: seq<T>, forbid : seq<T>)
+  // a match only counts if the character before or after is not in chars
+  method SearchAndReplaceAllWhole<T(==)>(source_in: seq<T>, old_str: seq<T>, new_str: seq<T>, chars : seq<T>)
     returns (o : seq<T>)
     requires 0 < |old_str|
   {
@@ -204,7 +206,7 @@ module StandardLibrary.String {
       invariant pos as nat <= |source|
       decreases |source| - pos as nat
     {
-      var res := SearchAndReplacePosNot(source, old_str, new_str, pos, forbid);
+      var res := SearchAndReplacePosWhole(source, old_str, new_str, pos, chars);
       if res.1.None? {
         SequenceIsSafeBecauseItIsInMemory(source);
         pos := |source| as uint64; // unneeded, but Dafny is dumb
