StandardLibrary/test/TestString.dfy
@@ -63,24 +63,24 @@ module TestStrings {
     expect actual == "rose_daisy is a rose_daisy is a rose_daisy";
   }
 
-  method {:test} TestSearchAndReplaceAllNotEasy()
+  method {:test} TestSearchAndReplaceAllWholeEasy()
   {
-    var actual := String.SearchAndReplaceAllNot("Koda is a Dog.", "Koda", "Robbie", String.AlphaNumericUnder);
+    var actual := String.SearchAndReplaceAllWhole("Koda is a Dog.", "Koda", "Robbie", String.AlphaNumericUnder);
     expect actual == "Robbie is a Dog.";
-    actual := String.SearchAndReplaceAllNot("Koda is a Dog.", "Dog", "good boy", String.AlphaNumericUnder);
+    actual := String.SearchAndReplaceAllWhole("Koda is a Dog.", "Dog", "good boy", String.AlphaNumericUnder);
     expect actual == "Koda is a good boy.";
-    actual := String.SearchAndReplaceAllNot("Koda is a Dog.", "Dog.", "good boy!", String.AlphaNumericUnder);
+    actual := String.SearchAndReplaceAllWhole("Koda is a Dog.", "Dog.", "good boy!", String.AlphaNumericUnder);
     expect actual == "Koda is a good boy!";
-    actual := String.SearchAndReplaceAllNot("Koda is a Dog.", "Robbie", "good boy!", String.AlphaNumericUnder);
+    actual := String.SearchAndReplaceAllWhole("Koda is a Dog.", "Robbie", "good boy!", String.AlphaNumericUnder);
     expect actual == "Koda is a Dog.";
-    actual := String.SearchAndReplaceAllNot("Koda is a Dog.", "Koda", "Koda", String.AlphaNumericUnder);
+    actual := String.SearchAndReplaceAllWhole("Koda is a Dog.", "Koda", "Koda", String.AlphaNumericUnder);
     expect actual == "Koda is a Dog.";
 
-    actual := String.SearchAndReplaceAllNot("A rose is a rose is a rose.", "rose", "daisy", String.AlphaNumericUnder);
+    actual := String.SearchAndReplaceAllWhole("A rose is a rose is a rose.", "rose", "daisy", String.AlphaNumericUnder);
     expect actual == "A daisy is a daisy is a daisy.";
-    actual := String.SearchAndReplaceAllNot("rose is a rose is a rose", "rose", "daisy", String.AlphaNumericUnder);
+    actual := String.SearchAndReplaceAllWhole("rose is a rose is a rose", "rose", "daisy", String.AlphaNumericUnder);
     expect actual == "daisy is a daisy is a daisy";
-    actual := String.SearchAndReplaceAllNot("rose is a rose is a rose", "rose", "rose_daisy", String.AlphaNumericUnder);
+    actual := String.SearchAndReplaceAllWhole("rose is a rose is a rose", "rose", "rose_daisy", String.AlphaNumericUnder);
     expect actual == "rose_daisy is a rose_daisy is a rose_daisy";
   }
 
@@ -112,53 +112,53 @@ module TestStrings {
     expect actual == ("Koda is a Dog.", Some(4));
   }
 
-  // in most cases SearchAndReplacePosNot is just like SearchAndReplacePos
-  method {:test} TestHasSearchAndReplacePosNotEasy()
+  // in most cases SearchAndReplacePosWhole is just like SearchAndReplacePos
+  method {:test} TestHasSearchAndReplacePosWholeEasy()
   {
-    var actual := String.SearchAndReplacePosNot("Koda is a Dog.", "Koda", "Robbie", 0, String.AlphaNumericUnder);
+    var actual := String.SearchAndReplacePosWhole("Koda is a Dog.", "Koda", "Robbie", 0, String.AlphaNumericUnder);
     expect actual == ("Robbie is a Dog.", Some(6));
-    actual := String.SearchAndReplacePosNot("Koda is a Dog.", "Koda", "Robbie", 1, String.AlphaNumericUnder);
+    actual := String.SearchAndReplacePosWhole("Koda is a Dog.", "Koda", "Robbie", 1, String.AlphaNumericUnder);
     expect actual == ("Koda is a Dog.", None);
 
-    actual := String.SearchAndReplacePosNot("Koda is a Dog.", "Dog", "good boy", 0, String.AlphaNumericUnder);
+    actual := String.SearchAndReplacePosWhole("Koda is a Dog.", "Dog", "good boy", 0, String.AlphaNumericUnder);
     expect actual == ("Koda is a good boy.", Some(18));
-    actual := String.SearchAndReplacePosNot("Koda is a Dog.", "Dog", "good boy", 10, String.AlphaNumericUnder);
+    actual := String.SearchAndReplacePosWhole("Koda is a Dog.", "Dog", "good boy", 10, String.AlphaNumericUnder);
     expect actual == ("Koda is a good boy.", Some(18));
-    actual := String.SearchAndReplacePosNot("Koda is a Dog.", "Dog", "good boy", 11, String.AlphaNumericUnder);
+    actual := String.SearchAndReplacePosWhole("Koda is a Dog.", "Dog", "good boy", 11, String.AlphaNumericUnder);
     expect actual == ("Koda is a Dog.", None);
 
-    actual := String.SearchAndReplacePosNot("Koda is a Dog.", "Dog.", "good boy!", 0, String.AlphaNumericUnder);
+    actual := String.SearchAndReplacePosWhole("Koda is a Dog.", "Dog.", "good boy!", 0, String.AlphaNumericUnder);
     expect actual == ("Koda is a good boy!", Some(19));
-    actual := String.SearchAndReplacePosNot("Koda is a Dog.", "Dog.", "good boy!", 10, String.AlphaNumericUnder);
+    actual := String.SearchAndReplacePosWhole("Koda is a Dog.", "Dog.", "good boy!", 10, String.AlphaNumericUnder);
     expect actual == ("Koda is a good boy!", Some(19));
-    actual := String.SearchAndReplacePosNot("Koda is a Dog.", "Dog.", "good boy!", 11, String.AlphaNumericUnder);
+    actual := String.SearchAndReplacePosWhole("Koda is a Dog.", "Dog.", "good boy!", 11, String.AlphaNumericUnder);
     expect actual == ("Koda is a Dog.", None);
 
-    actual := String.SearchAndReplacePosNot("Koda is a Dog.", "Robbie", "good boy!", 0, String.AlphaNumericUnder);
+    actual := String.SearchAndReplacePosWhole("Koda is a Dog.", "Robbie", "good boy!", 0, String.AlphaNumericUnder);
     expect actual == ("Koda is a Dog.", None);
-    actual := String.SearchAndReplacePosNot("Koda is a Dog.", "Koda", "Koda", 0, String.AlphaNumericUnder);
+    actual := String.SearchAndReplacePosWhole("Koda is a Dog.", "Koda", "Koda", 0, String.AlphaNumericUnder);
     expect actual == ("Koda is a Dog.", Some(4));
   }
 
   // when forbid comes in to play
-  method {:test} TestHasSearchAndReplacePosNotHard()
+  method {:test} TestHasSearchAndReplacePosWholeHard()
   {
-    var actual := String.SearchAndReplacePosNot("KodaisaDog", "Koda", "Robbie", 0, String.AlphaNumericUnder);
+    var actual := String.SearchAndReplacePosWhole("KodaisaDog", "Koda", "Robbie", 0, String.AlphaNumericUnder);
     expect actual == ("KodaisaDog", None);
-    actual := String.SearchAndReplacePosNot("KodaisaDog", "Dog", "Puppy", 1, String.AlphaNumericUnder);
+    actual := String.SearchAndReplacePosWhole("KodaisaDog", "Dog", "Puppy", 1, String.AlphaNumericUnder);
     expect actual == ("KodaisaDog", None);
-    actual := String.SearchAndReplacePosNot("Koda*isaDog", "Koda", "Robbie", 0, String.AlphaNumericUnder);
+    actual := String.SearchAndReplacePosWhole("Koda*isaDog", "Koda", "Robbie", 0, String.AlphaNumericUnder);
     expect actual == ("Robbie*isaDog", Some(6));
-    actual := String.SearchAndReplacePosNot("Kodaisa.Dog", "Dog", "Puppy", 1, String.AlphaNumericUnder);
+    actual := String.SearchAndReplacePosWhole("Kodaisa.Dog", "Dog", "Puppy", 1, String.AlphaNumericUnder);
     expect actual == ("Kodaisa.Puppy", Some(13));
   }
 
   // when forbid comes in to play
-  method {:test} TestHasSearchAndReplaceAllNotHard()
+  method {:test} TestHasSearchAndReplaceAllWholeHard()
   {
-    var actual := String.SearchAndReplaceAllNot("Koda1 Koda Koda2 Koda Koda3", "Koda", "Robbie", String.AlphaNumericUnder);
+    var actual := String.SearchAndReplaceAllWhole("Koda1 Koda Koda2 Koda Koda3", "Koda", "Robbie", String.AlphaNumericUnder);
     expect actual == "Koda1 Robbie Koda2 Robbie Koda3";
-    actual := String.SearchAndReplaceAllNot("Koda Koda1 Koda Koda2 Koda Koda3 Koda", "Koda", "Robbie", String.AlphaNumericUnder);
+    actual := String.SearchAndReplaceAllWhole("Koda Koda1 Koda Koda2 Koda Koda3 Koda", "Koda", "Robbie", String.AlphaNumericUnder);
     expect actual == "Robbie Koda1 Robbie Koda2 Robbie Koda3 Robbie";
   }
 
